src/Init/Data/BitVec/BasixAux.lean
@@ -1,0 +1,32 @@
+/-
+Copyright (c) 2024 Lean FRO, LLC. All rights reserved.
+Released under Apache 2.0 license as described in the file LICENSE.
+Authors: Joe Hendrix, Wojciech Nawrocki, Leonardo de Moura, Mario Carneiro, Alex Keizer, Harun Khan, Abdalrhman M Mohamed
+-/
+prelude
+import Init.Data.Fin.Basic
+
+set_option linter.missingDocs true
+
+namespace BitVec
+
+section Nat
+
+/-- The `BitVec` with value `i mod 2^n`. -/
+@[match_pattern]
+protected def ofNat (n : Nat) (i : Nat) : BitVec n where
+  toFin := Fin.ofNat' i (Nat.two_pow_pos n)
+
+instance instOfNat : OfNat (BitVec n) i where ofNat := .ofNat n i
+
+/-- Given a bitvector `x`, return the underlying `Nat`. This is O(1) because `BitVec` is a
+(zero-cost) wrapper around a `Nat`. -/
+protected def toNat (x : BitVec n) : Nat := x.toFin.val
+
+/-- Return the bound in terms of toNat. -/
+theorem isLt (x : BitVec w) : x.toNat < 2^w := x.toFin.isLt
+
+
+end Nat
+
+end BitVec
