src/Init/Data/UInt/Bitwise.lean
@@ -6,6 +6,7 @@ Authors: Markus Himmel
 prelude
 import Init.Data.UInt.Basic
 import Init.Data.Fin.Bitwise
+import Init.Data.BitVec.Lemmas
 
 set_option hygiene false in
 macro "declare_bitwise_uint_theorems" typeName:ident : command =>
@@ -17,8 +18,20 @@ namespace $typeName
 end $typeName
 )
 
-declare_bitwise_uint_theorems UInt8
 declare_bitwise_uint_theorems UInt16
 declare_bitwise_uint_theorems UInt32
 declare_bitwise_uint_theorems UInt64
 declare_bitwise_uint_theorems USize
+
+set_option hygiene false in
+macro "declare_new_bitwise_uint_theorems" typeName:ident : command =>
+`(
+namespace $typeName
+
+@[simp] protected theorem and_toNat (a b : $typeName) : (a &&& b).toNat = a.toNat &&& b.toNat := BitVec.toNat_and ..
+
+end $typeName
+)
+
+declare_new_bitwise_uint_theorems UInt8
+
